Update invariant proof

nola/iris/inv.v
@@ -1,22 +1,22 @@
 (** * Nola later-free invariant *)
 
 From nola.iris Require Export upd.
-From iris.algebra Require Import gmap_view gset coPset.
+From stdpp Require Export namespaces.
+From iris.algebra Require Import gset.
+From iris.base_logic.lib Require Import ghost_map wsat invariants.
 From iris.proofmode Require Import proofmode.
-From iris.base_logic.lib Require Export own wsat fancy_updates invariants.
 
 Implicit Type PROP : Type.
 
 (** ** Resources *)
 
-Class ninvGpreS PROP Σ :=
-  ninvGpreS_inv :: inG Σ (gmap_viewR positive (leibnizO PROP)).
 Class ninvGS PROP Σ := NinvGS {
-  ninv_inG :: ninvGpreS PROP Σ;
+  ninvGS_in :: ghost_mapG Σ positive (leibnizO PROP);
   ninv_name : gname;
 }.
-Definition ninvΣ PROP : gFunctors :=
-  GFunctor (gmap_viewRF positive (leibnizO PROP)).
+Class ninvGpreS PROP Σ :=
+  ninvGpreS_in :: ghost_mapG Σ positive (leibnizO PROP).
+Definition ninvΣ PROP : gFunctors := ghost_mapΣ positive (leibnizO PROP).
 #[export] Instance subG_ninvΣ `{!subG (ninvΣ PROP) Σ} : ninvGpreS PROP Σ.
 Proof. solve_inG. Qed.
 
@@ -25,31 +25,35 @@ Section ninv.
 
   (** ** Propositions *)
 
-  (** [ownNi]: Basic invariant token *)
-  Local Definition ownNi (i : positive) (P : PROP) : iProp Σ :=
-    own ninv_name (gmap_view_frag i DfracDiscarded (P : leibnizO _)).
+  (** [ownI]: Basic invariant token *)
+  Local Definition ownI (i : positive) (P : PROP) : iProp Σ :=
+    i ↪[ninv_name]□ P.
 
   (** [ninv]: Invariant token *)
   Local Definition ninv_def (N : namespace) (P : PROP) : iProp Σ :=
-    ∃ i, ⌜i ∈ (↑N:coPset)⌝ ∧ ownNi i P.
+    ∃ i, ⌜i ∈ (↑N:coPset)⌝ ∗ ownI i P.
   Local Definition ninv_aux : seal ninv_def. Proof. by eexists. Qed.
   Definition ninv := ninv_aux.(unseal).
   Local Lemma ninv_unseal : ninv = ninv_def.
   Proof. exact ninv_aux.(seal_eq). Qed.
+
+  (** [ninv] is timeless and persistent *)
   #[export] Instance ninv_timeless {N P} : Timeless (ninv N P).
   Proof. rewrite ninv_unseal. exact _. Qed.
   #[export] Instance ninv_persistent {N P} : Persistent (ninv N P).
   Proof. rewrite ninv_unseal. exact _. Qed.
 
   (** [ninv_wsat]: Invariant world satisfaction *)
-  Local Definition authNi (Ps : gmap positive (leibnizO PROP)) :=
-    own ninv_name (gmap_view_auth (DfracOwn 1) Ps).
+  Local Definition authI (I : gmap positive PROP) :=
+    ghost_map_auth ninv_name 1 I.
   Local Definition ninv_wsat_def (intp : PROP -d> iProp Σ) : iProp Σ :=
-    ∃ Ps, authNi Ps ∗ [∗ map] i ↦ P ∈ Ps, intp P ∗ ownD {[i]} ∨ ownE {[i]}.
+    ∃ I, authI I ∗ [∗ map] i ↦ P ∈ I, intp P ∗ ownD {[i]} ∨ ownE {[i]}.
   Local Definition ninv_wsat_aux : seal ninv_wsat_def. Proof. by eexists. Qed.
   Definition ninv_wsat := ninv_wsat_aux.(unseal).
   Local Lemma ninv_wsat_unseal : ninv_wsat = ninv_wsat_def.
   Proof. exact ninv_wsat_aux.(seal_eq). Qed.
+
+  (** [ninv_wsat] is non-expansive *)
   #[export] Instance ninv_wsat_ne : NonExpansive ninv_wsat.
   Proof. rewrite ninv_wsat_unseal. solve_proper. Qed.
   #[export] Instance ninv_wsat_proper : Proper ((≡) ==> (≡)) ninv_wsat.
@@ -57,107 +61,89 @@ Section ninv.
 
   (** ** Lemmas *)
 
-  (** ** Lookup in [authNi] *)
-  Local Lemma authNi_lookup {Ps i P} :
-    authNi Ps -∗ ownNi i P -∗ ⌜Ps !! i = Some P⌝.
+  (** Allocate [ownI] *)
+  Local Lemma ownI_alloc_rec {intp P N} :
+    (∀ i, ⌜i ∈ (↑N:coPset)⌝ → ownI i P -∗ intp P) -∗ ninv_wsat intp ==∗
+      ∃ i, ⌜i ∈ (↑N:coPset)⌝ ∗ ninv_wsat intp ∗ ownI i P.
   Proof.
-    iIntros "aPs iP". unfold authNi, ownNi. iCombine "aPs iP" as "eq".
-    rewrite own_valid gmap_view_both_validI bi.and_elim_r.
-    iDestruct "eq" as %eq. by apply leibniz_equiv in eq.
+    rewrite ninv_wsat_unseal. iIntros "→P [%I[I W]]".
+    iMod (own_unit (gset_disjUR positive) disabled_name) as "D".
+    iMod (own_updateP with "[$]") as (x) "[X D]".
+    { apply (gset_disj_alloc_empty_updateP_strong'
+        (λ i, I !! i = None ∧ i ∈ (↑N:coPset)))=> E.
+      case: (fresh_inv_name (E ∪ dom I) N)=>
+        [i[/not_elem_of_union[?/not_elem_of_dom ?]?]]. by exists i. }
+    iDestruct "X" as %[i[->[??]]].
+    iMod (ghost_map_insert_persist with "I") as "[I #i]"; [done|]. iModIntro.
+    iExists _. iFrame "i". iSplit; [done|]. iExists _. iFrame "I".
+    iApply (big_sepM_insert_2 with "[→P D]"); [|done]. iLeft.
+    iSplitR "D"; [|done]. by iApply "→P".
   Qed.
+  (** Turn [ownI] to [ninv] *)
+  Local Lemma ownI_ninv {i N P} : i ∈ (↑N:coPset) → ownI i P ⊢ ninv N P.
+  Proof. rewrite ninv_unseal. iIntros. iExists _. by iSplit. Qed.
+  (** Allocate [ninv] *)
+  Lemma ninv_alloc_rec {intp N P} :
+    (ninv N P -∗ intp P) =[ninv_wsat intp]=∗ ninv N P.
+  Proof.
+    iIntros "→P W".
+    iMod (ownI_alloc_rec with "[→P] W") as (i ?) "[W i]".
+    - iIntros (i ?) "i". iApply "→P". by iApply ownI_ninv.
+    - iModIntro. iFrame "W". by iApply ownI_ninv.
+  Qed.
+  Lemma ninv_alloc {intp N P} : intp P =[ninv_wsat intp]=∗ ninv N P.
+  Proof. iIntros "P W". iApply (ninv_alloc_rec with "[P] W"). by iIntros. Qed.
 
-  (** Open and close by [ownNi] *)
-  Local Lemma ownNi_open {intp i P} :
-    ownNi i P -∗ ownE {[i]} -∗ ninv_wsat intp -∗
+  (** Open by [ownI] *)
+  Local Lemma ownI_open {intp i P} :
+    ownI i P -∗ ownE {[i]} -∗ ninv_wsat intp -∗
       ninv_wsat intp ∗ intp P ∗ ownD {[i]}.
   Proof.
-    rewrite ninv_wsat_unseal. iIntros "iP Ei (%Ps & aPs & W)".
-    iDestruct (authNi_lookup with "aPs iP") as %eqP.
-    iDestruct (big_sepM_delete with "W") as "[[[$$]|Ei'] W]";
+    rewrite ninv_wsat_unseal. iIntros "i ? [%I[I W]]".
+    iDestruct (ghost_map_lookup with "I i") as %?.
+    iDestruct (big_sepM_lookup_acc with "W") as "[[[$$]|?] →W]";
       [done| |iDestruct (ownE_singleton_twice with "[$]") as "[]"].
-    iExists _. iFrame "aPs". iApply big_sepM_delete; [done|]. iFrame.
+    iExists _. iFrame "I". iApply "→W". by iRight.
   Qed.
-  Local Lemma ownNi_close {intp i P} :
-    ownNi i P -∗ intp P -∗ ownD {[i]} -∗ ninv_wsat intp -∗
+  (** Close by [ownI] *)
+  Local Lemma ownI_close {intp i P} :
+    ownI i P -∗ ownD {[i]} -∗ intp P -∗ ninv_wsat intp -∗
       ninv_wsat intp ∗ ownE {[i]}.
   Proof.
-    rewrite ninv_wsat_unseal. iIntros "iP P Di (%Ps & aPs & W)".
-    iDestruct (authNi_lookup with "aPs iP") as %eqP.
-    iDestruct (big_sepM_delete with "W") as "[[[_ Di']|$] W]";
+    rewrite ninv_wsat_unseal. iIntros "i ? ? [%I[I W]]".
+    iDestruct (ghost_map_lookup with "I i") as %?.
+    iDestruct (big_sepM_lookup_acc with "W") as "[[[_ ?]|$] →W]";
       [done|iDestruct (ownD_singleton_twice with "[$]") as %[]|].
-    iExists _. iFrame "aPs". iApply big_sepM_delete; [done|]. iFrame "W".
-    iLeft. iFrame.
+    iExists _. iFrame "I". iApply "→W". iLeft. iFrame.
   Qed.
-
-  (** Allocate [ownNi] *)
-  Local Lemma ownNi_alloc_rec {intp P} φ :
-    (∀ E : gset positive, ∃ i, i ∉ E ∧ φ i) →
-    (∀ i, ⌜φ i⌝ → ownNi i P -∗ intp P) -∗ ninv_wsat intp ==∗
-      ∃ i, ⌜φ i⌝ ∗ ninv_wsat intp ∗ ownNi i P.
-  Proof.
-    rewrite ninv_wsat_unseal. iIntros (fresh) "→P (%Ps & aPs & W)".
-    iMod (own_unit (gset_disjUR positive) disabled_name) as "?".
-    iMod (own_updateP with "[$]") as (I) "[X DI]".
-    { apply (gset_disj_alloc_empty_updateP_strong' (λ i, Ps !! i = None ∧ φ i)).
-      move=> E. case: (fresh (E ∪ dom Ps))=>
-        [i [/not_elem_of_union[? /not_elem_of_dom?] ?]]. by exists i. }
-    iDestruct "X" as %(i & -> & Psi & ?).
-    iMod (own_update with "aPs") as "[aPs iP]";
-      [by eapply (gmap_view_alloc _ i DfracDiscarded (P : leibnizO _))|].
-    iModIntro. iExists i. iSplit; [done|]. unfold ownNi.
-    iRevert "iP". iIntros "#iP". iFrame "iP". iExists _. iFrame "aPs".
-    iApply big_sepM_insert; [done|]. iFrame "W". iLeft. unfold ownD.
-    iFrame "DI". by iApply "→P".
-  Qed.
-
-  (** Get [ownE] out of the fancy update *)
-  Local Lemma fupd_accE {N E} : ↑N ⊆ E →
-    ⊢ |={E,E∖↑N}=> ownE (↑N) ∗ (ownE (↑N) ={E∖↑N,E}=∗ True).
+  (** Access [ownE] *)
+  Local Lemma ownE_acc {N E} :
+    ↑N ⊆ E →  ⊢ |={E,E∖↑N}=> ownE (↑N) ∗ (ownE (↑N) ={E∖↑N,E}=∗ True).
   Proof.
     rewrite fancy_updates.uPred_fupd_unseal /fancy_updates.uPred_fupd_def.
     move=> ?. iIntros "[$ E]". do 2 iModIntro.
     rewrite {1 4}(union_difference_L (↑ N) E); [|done].
     rewrite ownE_op; [|set_solver]. iDestruct "E" as "[$$]". by iIntros "$$".
   Qed.
-
   (** Access [ninv] *)
   Lemma ninv_acc {intp N E P} :
     ↑N ⊆ E → ninv N P =[ninv_wsat intp]{E,E∖↑N}=∗
       intp P ∗ (intp P =[ninv_wsat intp]{E∖↑N,E}=∗ True)%I.
   Proof.
-    move=> ?. rewrite ninv_unseal. iIntros "(%i & %iN & #iP) W".
-    iMod fupd_accE as "[N N→]"; [done|].
+    move=> ?. rewrite ninv_unseal. iIntros "[%i[% #i]] W".
+    iMod ownE_acc as "[N cl]"; [done|].
     rewrite {1 2}(union_difference_L {[i]} (↑N)); [|set_solver].
-    rewrite ownE_op; [|set_solver]. iDestruct "N" as "[i N∖i]".
-    iDestruct (ownNi_open with "iP i W") as "($ & $ & Di)". iModIntro.
-    iIntros "P W". iDestruct (ownNi_close with "iP P Di W") as "[$ i]".
-    iApply "N→". iFrame.
+    rewrite ownE_op; [|set_solver]. iDestruct "N" as "[E E']".
+    iDestruct (ownI_open with "i E W") as "[$[$ D]]". iModIntro.
+    iIntros "P W". iDestruct (ownI_close with "i D P W") as "[$ E]".
+    iApply "cl". iFrame.
   Qed.
-
-  (** Turn [ownNi] to [ninv] *)
-  Local Lemma ownNi_ninv {i N P} : i ∈ (↑N:coPset) → ownNi i P -∗ ninv N P.
-  Proof. rewrite ninv_unseal. iIntros. iExists _. by iSplit. Qed.
-
-  (** Allocate [ninv] *)
-  Lemma ninv_alloc_rec {intp N P} :
-    (ninv N P -∗ intp P) =[ninv_wsat intp]=∗ ninv N P.
-  Proof.
-    iIntros "→P W".
-    iMod (ownNi_alloc_rec (.∈ ↑N) with "[→P] W") as (i) "(%iN & W & iP)".
-    - move=> ?. apply fresh_inv_name.
-    - iIntros (? iN) "iP". iApply "→P". by iApply ownNi_ninv.
-    - iModIntro. iFrame "W". by iApply ownNi_ninv.
-  Qed.
-  Lemma ninv_alloc {intp N P} : intp P =[ninv_wsat intp]=∗ ninv N P.
-  Proof. iIntros "P W". iApply (ninv_alloc_rec with "[P] W"). by iIntros. Qed.
 End ninv.
 
-(** Allocate [∀ intp, ninv_wsat intp] *)
+(** Allocate [ninv_wsat] *)
 Lemma ninv_wsat_alloc `{!invGS_gen hlc Σ, !ninvGpreS PROP Σ} :
   ⊢ |==> ∃ _ : ninvGS PROP Σ, ∀ intp, ninv_wsat intp.
 Proof.
-  iMod (own_alloc (gmap_view_auth (DfracOwn 1) ∅)) as (γ) "a∅";
-    [by apply gmap_view_auth_valid|].
-  iModIntro. iExists (NinvGS _ _ _ γ). rewrite ninv_wsat_unseal. iIntros (?).
-  iExists ∅. rewrite big_opM_empty. iFrame.
+  iMod ghost_map_alloc_empty as (γ) "●". iModIntro. iExists (NinvGS _ _ _ γ).
+  rewrite ninv_wsat_unseal. iIntros (?). iExists ∅. by iFrame.
 Qed.
